theories/util/update.v
@@ -10,14 +10,14 @@ Implicit Type P Q: PROP.
 
 Lemma step_fupdN_nmono E m n P : m ≤ n → (|={E}▷=>^m P) -∗ (|={E}▷=>^n P).
 Proof.
-  move: n. elim m=> /=[|m']. { iIntros (? _) "?". by iApply step_fupdN_intro. }
-  move=> IH ? /succ_le [n'[->Le]]/=. iIntros "?". by iApply IH.
+  move: n. elim: m=> /=[|?]; [iIntros; by iApply step_fupdN_intro|].
+  move=> IH ? /succ_le [?[->Le]]/=. iIntros "?". by iApply IH.
 Qed.
 
 Lemma step_fupdN_combine n E P Q :
   (|={E}▷=>^n P) -∗ (|={E}▷=>^n Q) -∗ (|={E}▷=>^n (P ∗ Q)).
 Proof.
-  elim n=> /=[|?]; [iIntros; by iFrame|]. iIntros (IH) ">UpdP >UpdQ !>!>".
+  elim: n=> /=[|?]; [iIntros; by iFrame|]. iIntros (IH) ">UpdP >UpdQ !>!>".
   by iMod (IH with "UpdP UpdQ").
 Qed.
 
